Table/Demo_prefilled.lean
@@ -1,0 +1,244 @@
+import Table.Widgets
+import Table.Proofs
+
+#print Header
+#print Schema
+#check Table
+#check Row
+#check Cell
+
+/-
+| Number |       Content       |
+--------------------------------
+| 9      | Rationals and reals |
+| 10     | Metaprogramming     |
+-/
+
+def myTable :
+  Table [("Number", Nat), ("Content", String)] :=
+Table.mk [
+  (Row.cons (Cell.val 9)
+    (Row.cons (Cell.val "Rationals and Reals")
+      Row.nil))
+]
+-- Table.mk
+--       [ /[9             ,  "Rationals and Reals" ],
+--         /[10            ,  "Metaprogramming"]
+--       ]
+
+def myTableDropped := dropColumns myTable A[⟨"Number", by name⟩]
+
+#table myTable
+
+#check ActionList
+
+/- Demo! -/
+
+inductive GradeMode
+| ABC
+| SNC
+deriving DecidableEq
+instance : ToString GradeMode := ⟨λ | .ABC => "ABC" | .SNC => "SNC"⟩
+
+def roster :
+  Table [("Name", String), ("Banner ID", String), ("Grade Mode", GradeMode)] :=
+Table.mk [
+  /[ "Alice", "B00000001", GradeMode.ABC ],
+  /[ "Bob"  , "B00000002", GradeMode.ABC ],
+  /[ "Carol", "B00000003", GradeMode.SNC ],
+  /[ "Dave" , "B00000004", GradeMode.ABC ],
+  /[ "Eve"  , "B00000005", GradeMode.SNC ],
+  /[ "Frank", "B00000006", GradeMode.ABC ],
+  /[ "Grace", "B00000007", GradeMode.SNC ]
+]
+
+#table roster
+
+def disambiguationTable : Table [("Name", String), ("Anonymous ID", Nat)] :=
+Table.mk [
+  /[ "Grace", 18637600 ],
+  /[ "Carol", 19511951 ],
+  /[ "Bob"  , 27182818 ],
+  /[ "Eve"  , 29109101 ],
+  /[ "Alice", 31415926 ],
+  /[ "Dave" , 32033030 ],
+  /[ "Frank", 40186310 ]
+]
+
+#table disambiguationTable
+
+inductive LetterGrade
+| A | B | C | S | NC
+deriving DecidableEq
+instance : ToString LetterGrade :=
+  ⟨λ | .A => "A" | .B => "B" | .C => "C" | .S => "S" | .NC => "NC"⟩
+
+def grades :
+  Table [("Anonymous ID", Nat),
+         ("hw1", Nat),
+         ("hw2", Nat),
+         ("midterm", Nat),
+         ("hw3", Nat),
+         ("final", Nat),
+         ("project", LetterGrade)] :=
+Table.mk [
+  /[ 31415926, 95 , 83, 85, 91 , 88, LetterGrade.A ],
+  /[ 32033030, 92 , 98 , 90, 90 , 91, LetterGrade.A ],
+  /[ 27182818, 75 , EMP, 78, 88 , 83, LetterGrade.B ],
+  /[ 29109101, 97 , 92 , 91, EMP, 90, LetterGrade.B ],
+  /[ 19511951, EMP, 83 , 70, 84 , 74, LetterGrade.C ],
+  /[ 18637600, 92 , 96 , 89, 97 , 91, LetterGrade.A ],
+  /[ 40186310, 86 , 91 , 77, 85 , 81, LetterGrade.C ]
+]
+
+#table grades
+
+-- Find the average prior performance of students by project grade:
+
+def oAverage (xs : List $ Option Nat) : Option Nat := some $
+  List.foldl (λ acc => λ | none => acc | some x => x + acc) 0 xs / xs.length
+
+def projectExamGrades :
+  Table [("project", LetterGrade), ("mt_avg", Nat), ("final_avg", Nat)] :=
+  pivotTable
+        grades
+        [⟨("project", _), by header⟩]
+        (by inst)
+        [⟨("mt_avg", _), ⟨("midterm", _), by header⟩, oAverage⟩,
+         ⟨("final_avg", _), ⟨("final", _), by header⟩, oAverage⟩]
+
+#table projectExamGrades
+    
+-- Try to match up the roster with anonymous IDs
+
+def studentsWithIdsBasic := hcat roster disambiguationTable
+
+#table disambiguationTable
+#table studentsWithIdsBasic
+
+def studentsWithIds :=
+  leftJoin roster
+           disambiguationTable
+           A[⟨("Name", _), inferInstance, by header, by header⟩]
+
+#table studentsWithIds
+
+-- Join the IDed roster with grade data; in the end, we only need Banner IDs
+
+def studentsWithIdsAndGrades :=
+  leftJoin studentsWithIds
+           grades
+           A[⟨("Anonymous ID", _), inferInstance, by header, by header⟩]
+
+#table studentsWithIdsAndGrades
+
+def gradesByBannerID :=
+  dropColumns studentsWithIdsAndGrades
+    A[⟨"Anonymous ID", by name⟩, ⟨"Name", by name⟩]
+
+#table gradesByBannerID
+
+-- Fill in 0s for missing grades
+
+def gradesFilledIn :=
+  List.foldl (λ acc x =>
+    fillna acc x 0
+  ) gradesByBannerID
+  [⟨"hw1", by header⟩, ⟨"hw2", by header⟩, ⟨"hw3", by header⟩,
+   ⟨"midterm", by header⟩, ⟨"final", by header⟩]
+
+#table gradesFilledIn
+
+-- Compute final grades
+
+/- USE THIS IF NOT DOING FILLNA:
+def computeGrade (r : Row (schema studentsWithIdsAndGrades))
+                 (_ : Fin (nrows studentsWithIdsAndGrades)) :=
+  let hw1 := (getValue r "hw1" (by header)).getD 0
+  let hw2 := (getValue r "hw2" (by header)).getD 0
+  let hw3 := (getValue r "hw3" (by header)).getD 0
+  let midterm := (getValue r "midterm" (by header)).getD 0
+  let final := (getValue r "final" (by header)).getD 0
+  let project :=
+    match getValue r "project" (by header) with
+    | some LetterGrade.A => 95
+    | some LetterGrade.B => 85
+    | some LetterGrade.C => 75
+    | _ => 0
+  let gradeMode := getValue r "Grade Mode" (by header)
+  let numericGrade :=
+    ((hw1 + hw2 + hw3) + 2 * midterm + 2 * final + 3 * project) / 10
+  let finalGrade :=
+    match gradeMode with
+    | some GradeMode.ABC =>
+      if numericGrade ≥ 90
+      then LetterGrade.A
+      else if numericGrade ≥ 80
+      then LetterGrade.B
+      else if numericGrade ≥ 70
+      then LetterGrade.C
+      else LetterGrade.NC
+    | _ => if numericGrade ≥ 70 then LetterGrade.S else LetterGrade.NC
+  match getValue (τ := String) r "Banner ID" (by header) with
+  | some bid => /["Banner ID" := bid, "Grade" := finalGrade]
+  | _        => /["Banner ID" := EMP, "Grade" := finalGrade]
+-/
+
+def computeGrade (r : Row (schema gradesFilledIn))
+                 (_ : Fin (nrows gradesFilledIn)) :=
+  let hw1 := (getValue r "hw1" (by header)).getD 0
+  let hw2 := (getValue r "hw2" (by header)).getD 0
+  let hw3 := (getValue r "hw3" (by header)).getD 0
+  let midterm := (getValue r "midterm" (by header)).getD 0
+  let final := (getValue r "final" (by header)).getD 0
+  let project :=
+    match getValue r "project" (by header) with
+    | some LetterGrade.A => 95
+    | some LetterGrade.B => 85
+    | some LetterGrade.C => 75
+    | _ => 0
+  let gradeMode := getValue r "Grade Mode" (by header)
+  let numericGrade :=
+    ((hw1 + hw2 + hw3) + 2 * midterm + 2 * final + 3 * project) / 10
+  let finalGrade :=
+    match gradeMode with
+    | some GradeMode.ABC =>
+      if numericGrade ≥ 90
+      then LetterGrade.A
+      else if numericGrade ≥ 80
+      then LetterGrade.B
+      else if numericGrade ≥ 70
+      then LetterGrade.C
+      else LetterGrade.NC
+    | _ => if numericGrade ≥ 70 then LetterGrade.S else LetterGrade.NC
+  match getValue (τ := String) r "Banner ID" (by header) with
+  | some bid => /["Banner ID" := bid, "Grade" := finalGrade]
+  | _        => /["Banner ID" := EMP, "Grade" := finalGrade]
+
+def finalGrades := select gradesFilledIn computeGrade
+
+#table gradesFilledIn
+
+#table finalGrades
+
+-- Group student grades by project grades:
+
+def groupedByProject := groupBySubtractive grades ⟨"project", by header⟩
+
+#table groupedByProject
+
+#check groupBySubtractive_spec7
+#check getColumn2_spec2
+
+-- The result of doing this kind of "grouping" should only ever reduce the
+-- number of rows in the resulting (outer) table:
+
+theorem nrows_groupBySubtractive {η τ} [DecidableEq η] [DecidableEq τ]
+  {schema : @Schema η} (t : Table schema) (c : (c : η) × schema.HasCol (c, τ)) :
+  nrows (groupBySubtractive t c) ≤ nrows t :=
+  by
+    have h_spec := groupBySubtractive_spec7 t c
+    rw [h_spec]
+    have h := getColumn2_spec2 t c.fst c.snd
+    rw [←h]
+    apply List.length_unique_le
