Table/OldTests.lean
@@ -1,0 +1,189 @@
+import Table.API
+
+macro "header" : tactic => `(repeat ((try apply Schema.HasCol.hd) <;> (apply Schema.HasCol.tl)))
+macro "name" : tactic => `(repeat ((try apply Schema.HasName.hd) <;> (apply Schema.HasName.tl)))
+
+universe u_η
+universe u
+variable {η : Type u_η} [dec_η : DecidableEq η] {schema : @Schema η}
+
+#check Cell "hi" Nat
+
+def x : Cell "hi" Nat := Cell.val 42
+
+-- Implementation of a table string-representation function (provided all τs in
+-- the schema have ToString instances):
+instance : ToString (@Row η dec_η []) where
+  toString := λ_ => ""
+
+instance {η nm τ} {xs : @Schema η} [ToString τ] [DecidableEq η] [ToString (Row xs)] : ToString (Row ((nm, τ) :: xs)) where
+  toString := λ(Row.cons cell d) =>
+                let s := match cell.toOption with
+                         | some v => toString v
+                         | none   => "[empty]";
+                let s_d := toString d; 
+                s ++ (if s_d = "" then "" else "\t|\t" ++ s_d)
+
+def Row.repr [ToString (Row schema)] (r : Row schema) := toString r
+
+instance {η} {schema : @Schema η} [ToString η] [DecidableEq η] [inst : ToString (Row schema)] : ToString (Table schema) where
+  toString := λ t =>
+  List.foldr (λ (nm, _) acc => ToString.toString nm ++ (if acc = "" then "" else "\t|\t") ++ acc) "" schema
+    ++ "\n"
+    ++ List.foldr (λ r acc => inst.toString r ++ "\n" ++ acc) "" t.rows
+
+def Table.repr [ToString (Table schema)] (t : Table schema) := toString t
+
+#eval Row.repr (Row.cons x (Row.cons x Row.nil))
+
+-- This could probably use some syntactic sugar...
+def t1 : Table [("prof", String), ("course", Nat), ("taught", Bool)] :=
+  -- Can simplify this by just using Table.mk
+  addRows
+    (emptyTable |> (λ t => addColumn t "prof" [])
+                |> (λ t => addColumn t "course" [])
+                |> (λ t => addColumn t "taught" []))
+    [Row.cons (Cell.val "Kaynar") (Row.cons (Cell.val 15122) (Row.cons (Cell.val true) Row.nil)),
+      Row.cons (Cell.val "Crary") (Row.cons (Cell.val 15150) (Row.cons (Cell.val true) Row.nil)),
+      Row.cons (Cell.val "Erdmann") (Row.cons (Cell.val 15150) (Row.cons (Cell.val false) Row.nil)),
+      Row.cons (Cell.val "Cervesato") (Row.cons (Cell.val 15122) (Row.cons (Cell.val false) Row.nil))]
+
+#eval Table.repr t1
+#reduce t1
+
+infixr:50 "||" => Row.cons
+notation "**|" => Row.nil
+notation "/[" elem "]/" => Cell.val elem
+notation "/[_]/" => Cell.emp
+
+def t2 : Table [("prof", String), ("course", Nat), ("taught", Bool)] :=
+  Table.mk
+    [
+      /[ "Lewis" ]/         || /[_]/      || /[ true ]/  || **|,
+      /[ "Krishnamurthi" ]/ || /[ 1730 ]/ || /[ false ]/ || **|
+      ]
+
+def row1 := getRow t2 1 (by simp)
+
+def joined := vcat t1 t2
+#eval joined
+#reduce joined
+
+#reduce selectColumns3 t2 [⟨"prof", (by name)⟩, ⟨"course", (by name)⟩]
+#reduce @selectColumns3 String
+                        inferInstance
+                        [("prof", String), ("course", Nat), ("taught", Bool)] t2 [⟨"prof", Schema.HasName.hd⟩]
+#reduce Row.pick (Row.append
+        (@Row.singleCell String _ "pi" (List Nat) [3,1,4,1,5])
+        (@Row.singleCell String _ "age" Nat 20)) [⟨"pi", by name⟩]
+
+def schoolIded := addColumn joined "school" ["CMU", "CMU", "CMU", "CMU", "Brown", "Brown"]
+#check schoolIded
+
+#reduce getValue (List.head schoolIded.rows _) "course" (by header)
+
+#reduce selectRows1 schoolIded [⟨3, _⟩, ⟨4, _⟩]
+#reduce schoolIded |> (λ t => selectRows1 t [⟨1, _⟩, ⟨4, _⟩])
+                   |> (λ t => selectColumns1 t [true, false, false, true])
+
+-- Testing, etc.
+#reduce addRows (addColumn emptyTable "name" []) [Row.singleCell "hello"]
+-- FIX?ME: the Lean m4 update broke this (used to be no need for explicit args)
+-- More generally, type-class resolution seems to be kind of broken right now.
+-- (Haven't checked this since moving away from type classes)
+#reduce getValue (Row.append
+        (@Row.singleCell String _ "pi" (List Nat) [3,1,4,1,5])
+        (@Row.singleCell String _ "age" Nat 20))
+        "age" (by header)
+
+#eval @update _ _ _ [⟨("prof", String), by header⟩] t2 (λ r => @Row.singleCell _ _ "prof" String "Rob")
+-- #eval update _ t2 (λ r => @Row.singleCell _ _ "prof" String "Rob")
+
+#eval fillna joined ⟨"course", (by header)⟩ 1951
+
+def departments : Table [("Department ID", Nat),
+                         ("Department Name", String)] :=
+Table.mk [
+  /[31]/ || /["Sales"]/       || **|,
+  /[33]/ || /["Engineering"]/ || **|,
+  /[34]/ || /["Clerical"]/    || **|,
+  /[35]/ || /["Marketing"]/   || **|
+]
+
+def dupDepts := addRows departments [/[31]/ || /["Information"]/ || **|,
+                                     /[33]/ || /["Security"]/ || **|,
+                                     /[34]/ || /["Parallelism"]/ || **|,
+                                     /[35]/ || /["Functionalism"]/ || **|]
+def dupDepts' := addColumn dupDepts "Number" [89, 7, 25, 27, 4, 3, 24, 1]
+
+#eval head departments ⟨-2, sorry⟩
+#reduce dropColumn joined ⟨"taught", by name⟩
+#eval tsort dupDepts' ⟨"Number", by header⟩ true
+#eval sortByColumns dupDepts' [⟨("Department ID", _), by header, by infer_instance⟩,
+                               ⟨("Number", _), by header, by infer_instance⟩]
+
+
+#reduce (count joined ⟨"course", by header⟩)
+def merge : Option Nat → List (Option Nat) → Row [("Parity", Bool), ("Length", Nat)]
+| (some n), xs =>
+  let xs_sum := xs.foldl (λ | acc, none => acc
+                            | acc, (some n) => acc + n) 0
+  Row.cons (Cell.val (n = 1)) (Row.cons (Cell.val xs_sum) Row.nil)
+| none, _ => Row.cons Cell.emp (Row.cons Cell.emp Row.nil)
+
+-- FIXME: allowing different η' broke something
+#reduce @groupBy _ _ _ String _ _ _ _ _ departments (λ r => (getValue r "Department ID" (by header)).map (λ (x : Nat) => Nat.mod x 2))
+                            (λ r => (getValue r "Department Name" (by header)).map (λ (x : String) => x.length))
+  (λ | (some n), xs =>
+        let xs_sum := xs.foldl (λ | acc, none => acc
+                                  | acc, (some n) => acc + n) 0
+        Row.cons (Cell.val (decide (n = 1))) (Row.cons (Cell.val xs_sum) Row.nil)
+     | none, _ => Row.cons Cell.emp (Row.cons Cell.emp Row.nil))
+
+def listTable : Table [("Number", String), ("Digits", List Nat)] :=
+Table.mk [
+  /["pi"]/ || /[[3,1,4,1,5]]/ || **|,
+  /["e"]/  || /[[2,7,1,8,2]]/ || **|
+]
+
+#reduce flattenOne listTable ⟨"Digits", by header⟩
+
+#eval bin departments ⟨"Department ID", by header⟩ 2
+
+def gradebookTable : Table [("name", ULift String),
+                            ("age", ULift Nat),
+                            ("quizzes", Table [("quiz#", {n : Nat // 1 ≤ n ∧ n ≤ 4}),
+                                               ("grade", Nat)]),
+                            ("midterm", ULift Nat),
+                            ("final", ULift Nat)] :=
+Table.mk [
+  /[ULift.up "Bob"]/ ||
+  /[ULift.up 12]/ ||
+  /[Table.mk [/[⟨1, by simp⟩]/ || /[8]/ || **|,
+              /[⟨2, by simp⟩]/ || /[9]/ || **|,
+              /[⟨3, by simp⟩]/ || /[7]/ || **|,
+              /[⟨4, by simp⟩]/ || /[9]/ || **|]]/ ||
+  /[ULift.up 77]/ ||
+  /[ULift.up 87]/ || **|,
+
+  /[ULift.up "Alice"]/ ||
+  /[ULift.up 17]/ ||
+  /[Table.mk [/[⟨1, by simp⟩]/ || /[6]/ || **|,
+              /[⟨2, by simp⟩]/ || /[8]/ || **|,
+              /[⟨3, by simp⟩]/ || /[8]/ || **|,
+              /[⟨4, by simp⟩]/ || /[7]/ || **|]]/ ||
+  /[ULift.up 88]/ ||
+  /[ULift.up 85]/ || **|,
+
+  /[ULift.up "Eve"]/ ||
+  /[ULift.up 13]/ ||
+  /[Table.mk [/[⟨1, by simp⟩]/ || /[7]/ || **|,
+              /[⟨2, by simp⟩]/ || /[9]/ || **|,
+              /[⟨3, by simp⟩]/ || /[8]/ || **|,
+              /[⟨4, by simp⟩]/ || /[8]/ || **|]]/ ||
+  /[ULift.up 84]/ ||
+  /[ULift.up 77]/ || **|
+  
+]
+
+#eval Table.repr gradebookTable
