Table/deleteme.lean
@@ -1,0 +1,646 @@
+import Lean
+import Lean.Util.CollectLevelParams
+import Lean.Elab.DeclUtil
+import Lean.Elab.DefView
+import Lean.Elab.Inductive
+import Lean.Elab.Structure
+import Lean.Elab.MutualDef
+import Lean.Elab.DeclarationRange
+namespace Lean.Elab.Command
+
+open Meta
+
+instance : ToString CtorView := ⟨λ (v : CtorView) =>
+  "{ref: " ++ toString v.ref ++ "}\n" ++
+  "{mods: " ++ toString v.modifiers ++ "}\n" ++
+  "{decl: " ++ toString v.declName ++ "}\n" ++
+  "{type?: " ++ toString v.type? ++ "}\n"
+    ⟩
+
+/-
+leading_parser "inductive " >> declId >> optDeclSig >> optional ":=" >> many ctor
+leading_parser atomic (group ("class " >> "inductive ")) >> declId >> optDeclSig >> optional ":=" >> many ctor >> optDeriving
+-/
+private def badInductiveSyntaxToView (modifiers : Modifiers) (decl : Syntax) : CommandElabM InductiveView := do
+  checkValidInductiveModifier modifiers
+  let (binders, type?) := expandOptDeclSig decl[2]
+  let declId           := decl[1]
+  let ⟨name, declName, levelNames⟩ ← expandDeclId declId modifiers
+  addDeclarationRanges declName decl
+  let ctors      ← decl[3].getArgs.mapM fun ctor => withRef ctor do
+    -- def ctor := leading_parser " | " >> declModifiers >> ident >> optDeclSig
+    let ctorModifiers ← elabModifiers ctor[1]
+    if ctorModifiers.isPrivate && modifiers.isPrivate then
+      throwError "invalid 'private' constructor in a 'private' inductive datatype"
+    if ctorModifiers.isProtected && modifiers.isPrivate then
+      throwError "invalid 'protected' constructor in a 'private' inductive datatype"
+    checkValidCtorModifier ctorModifiers
+    let ctorName := ctor.getIdAt 2
+    let ctorName := declName ++ ctorName
+    let ctorName ← withRef ctor[2] <| applyVisibility ctorModifiers.visibility ctorName
+    let (binders, type?) := expandOptDeclSig ctor[3]
+    addDocString' ctorName ctorModifiers.docString?
+    addAuxDeclarationRanges ctorName ctor ctor[2]
+    return { ref := ctor, modifiers := ctorModifiers, declName := ctorName, binders := binders, type? := type? : CtorView }
+  let mut computedFields := #[]
+  let mut classes := #[]
+  if decl.getNumArgs == 5 then
+    -- TODO: remove after stage0 update
+    classes ← getOptDerivingClasses decl[4]
+  else
+    computedFields ← (decl[4].getOptional?.map (·[1].getArgs) |>.getD #[]).mapM fun cf => withRef cf do
+      return { ref := cf, modifiers := cf[0], fieldId := cf[1].getId, type := ⟨cf[3]⟩, matchAlts := ⟨cf[4]⟩ }
+    classes ← getOptDerivingClasses decl[6]
+  return {
+    ref             := decl
+    shortDeclName   := name
+    derivingClasses := classes
+    declId, modifiers, declName, levelNames
+    binders, type?, ctors
+    computedFields
+  }
+
+private partial def elabHeaderAux (views : Array InductiveView) (i : Nat) (acc : Array ElabHeaderResult) : TermElabM (Array ElabHeaderResult) :=
+  Term.withAutoBoundImplicitForbiddenPred (fun n => views.any (·.shortDeclName == n)) do
+    if h : i < views.size then
+      let view := views.get ⟨i, h⟩
+      let acc ← Term.withAutoBoundImplicit <| Term.elabBinders view.binders.getArgs fun params => do
+        match view.type? with
+        | none         =>
+          let u ← mkFreshLevelMVar
+          let type := mkSort u
+          Term.synthesizeSyntheticMVarsNoPostponing
+          Term.addAutoBoundImplicits' params type fun params type => do
+            return acc.push { lctx := (← getLCtx), localInsts := (← getLocalInstances), params, type, view }
+        | some typeStx =>
+          let (type, _) ← Term.withAutoBoundImplicit do
+            let type ← Term.elabType typeStx
+            unless (← isTypeFormerType type) do
+              throwErrorAt typeStx "invalid inductive type, resultant type is not a sort"
+            Term.synthesizeSyntheticMVarsNoPostponing
+            let indices ← Term.addAutoBoundImplicits #[]
+            return (← mkForallFVars indices type, indices.size)
+          Term.addAutoBoundImplicits' params type fun params type => do
+            trace[Elab.inductive] "header params: {params}, type: {type}"
+            return acc.push { lctx := (← getLCtx), localInsts := (← getLocalInstances), params, type, view }
+      elabHeaderAux views (i+1) acc
+    else
+      return acc
+
+private def elabHeader (views : Array InductiveView) : TermElabM (Array ElabHeaderResult) := do
+  let rs ← elabHeaderAux views 0 #[]
+  -- if rs.size > 1 then
+    -- checkUnsafe rs
+    -- let numParams ← checkNumParams rs
+    -- checkHeaders rs numParams 0 none
+  return rs
+
+private def mkTypeFor (r : ElabHeaderResult) : TermElabM Expr := do
+  withLCtx r.lctx r.localInsts do
+    mkForallFVars r.params r.type
+
+private partial def withInductiveLocalDecls (rs : Array ElabHeaderResult) (x : Array Expr → Array Expr → TermElabM α) : TermElabM α := do
+  let namesAndTypes ← rs.mapM fun r => do
+    let type ← mkTypeFor r
+    pure (r.view.declName, r.view.shortDeclName, type)
+  let r0     := rs[0]!
+  let params := r0.params
+  withLCtx r0.lctx r0.localInsts <| withRef r0.view.ref do
+    let rec loop (i : Nat) (indFVars : Array Expr) := do
+      if h : i < namesAndTypes.size then
+        let (declName, shortDeclName, type) := namesAndTypes.get ⟨i, h⟩
+        Term.withAuxDecl shortDeclName type declName fun indFVar => loop (i+1) (indFVars.push indFVar)
+      else
+        x params indFVars
+    loop 0 #[]
+
+private def withExplicitToImplicit (xs : Array Expr) (k : TermElabM α) : TermElabM α := do
+  let mut toImplicit := #[]
+  for x in xs do
+    if (← getFVarLocalDecl x).binderInfo.isExplicit then
+      toImplicit := toImplicit.push (x.fvarId!, BinderInfo.implicit)
+  withNewBinderInfos toImplicit k
+
+private def isInductiveFamily (numParams : Nat) (indFVar : Expr) : TermElabM Bool := do
+  let indFVarType ← inferType indFVar
+  forallTelescopeReducing indFVarType fun xs _ =>
+    return xs.size > numParams
+
+private def getArrowBinderNames (type : Expr) : Array Name :=
+  go type #[]
+where
+  go (type : Expr) (acc : Array Name) : Array Name :=
+    match type with
+    | .forallE n _ b _ => go b (acc.push n)
+    | .mdata _ b       => go b acc
+    | _ => acc
+
+private def replaceArrowBinderNames (type : Expr) (newNames : Array Name) : Expr :=
+  go type 0
+where
+  go (type : Expr) (i : Nat) : Expr :=
+    if i < newNames.size then
+      match type with
+      | .forallE n d b bi =>
+        if n.hasMacroScopes then
+          mkForall newNames[i]! bi d (go b (i+1))
+        else
+          mkForall n bi d (go b (i+1))
+      | _ => type
+    else
+      type
+
+private def reorderCtorArgs (ctorType : Expr) : MetaM Expr := do
+  forallTelescopeReducing ctorType fun as type => do
+    /- `type` is of the form `C ...` where `C` is the inductive datatype being defined. -/
+    let bs := type.getAppArgs
+    let mut as  := as
+    let mut bsPrefix := #[]
+    for b in bs do
+      unless b.isFVar && as.contains b do
+        break
+      let localDecl ← getFVarLocalDecl b
+      if localDecl.binderInfo.isExplicit then
+        break
+      unless localDecl.userName.hasMacroScopes do
+        break
+      if (← localDeclDependsOnPred localDecl fun fvarId => as.any fun p => p.fvarId! == fvarId) then
+        break
+      bsPrefix := bsPrefix.push b
+      as := as.erase b
+    if bsPrefix.isEmpty then
+      return ctorType
+    else
+      let r ← mkForallFVars (bsPrefix ++ as) type
+      /- `r` already contains the resulting type.
+         To be able to produce more better error messages, we copy the first `bsPrefix.size` binder names from `C` to `r`.
+         This is important when some of contructor parameters were inferred using the auto-bound implicit feature.
+         For example, in the following declaration.
+         ```
+          inductive Member : α → List α → Type u
+            | head : Member a (a::as)
+            | tail : Member a bs → Member a (b::bs)
+         ```
+         if we do not copy the binder names
+         ```
+         #check @Member.head
+         ```
+         produces `@Member.head : {x : Type u_1} → {a : x} → {as : List x} → Member a (a :: as)`
+         which is correct, but a bit confusing. By copying the binder names, we obtain
+         `@Member.head : {α : Type u_1} → {a : α} → {as : List α} → Member a (a :: as)`
+       -/
+      let C := type.getAppFn
+      let binderNames := getArrowBinderNames (← instantiateMVars (← inferType C))
+      return replaceArrowBinderNames r binderNames[:bsPrefix.size]
+
+private def elabCtors (indFVars : Array Expr) (indFVar : Expr) (params : Array Expr) (r : ElabHeaderResult) : TermElabM (List Constructor) := withRef r.view.ref do
+  let indFamily ← isInductiveFamily params.size indFVar
+  r.view.ctors.toList.mapM fun ctorView =>
+    Term.withAutoBoundImplicit <| Term.elabBinders ctorView.binders.getArgs fun ctorParams =>
+      withRef ctorView.ref do
+        let rec elabCtorType (k : Expr → TermElabM Constructor) : TermElabM Constructor := do
+          match ctorView.type? with
+          | none          =>
+            if indFamily then
+              throwError "constructor resulting type must be specified in inductive family declaration"
+            k <| mkAppN indFVar params
+          | some ctorType =>
+            let type ← Term.elabType ctorType
+            trace[Elab.inductive] "elabType {ctorView.declName} : {type} "
+            Term.synthesizeSyntheticMVars (mayPostpone := true)
+            let type ← instantiateMVars type
+            let type ← checkParamOccs type
+            forallTelescopeReducing type fun _ resultingType => do
+              unless resultingType.getAppFn == indFVar do
+                throwError "unexpected constructor resulting type{indentExpr resultingType}"
+              unless (← isType resultingType) do
+                throwError "unexpected constructor resulting type, type expected{indentExpr resultingType}"
+            k type
+        elabCtorType fun type => do
+          Term.synthesizeSyntheticMVarsNoPostponing
+          let ctorParams ← Term.addAutoBoundImplicits ctorParams
+          let except (mvarId : MVarId) := ctorParams.any fun ctorParam => ctorParam.isMVar && ctorParam.mvarId! == mvarId
+          /-
+            We convert metavariables in the resulting type info extra parameters. Otherwise, we would not be able to elaborate
+            declarations such as
+            ```
+            inductive Palindrome : List α → Prop where
+              | nil      : Palindrome [] -- We would get an error here saying "failed to synthesize implicit argument" at `@List.nil ?m`
+              | single   : (a : α) → Palindrome [a]
+              | sandwich : (a : α) → Palindrome as → Palindrome ([a] ++ as ++ [a])
+            ```
+            We used to also collect unassigned metavariables on `ctorParams`, but it produced counterintuitive behavior.
+            For example, the following declaration used to be accepted.
+            ```
+            inductive Foo
+            | bar (x)
+
+            #check Foo.bar
+            -- @Foo.bar : {x : Sort u_1} → x → Foo
+            ```
+            which is also inconsistent with the behavior of auto implicits in definitions. For example, the following example was never accepted.
+            ```
+            def bar (x) := 1
+            ```
+          -/
+          let extraCtorParams ← Term.collectUnassignedMVars (← instantiateMVars type) #[] except
+          trace[Elab.inductive] "extraCtorParams: {extraCtorParams}"
+          /- We must abstract `extraCtorParams` and `ctorParams` simultaneously to make
+             sure we do not create auxiliary metavariables. -/
+          let type  ← mkForallFVars (extraCtorParams ++ ctorParams) type
+          let type ← reorderCtorArgs type
+          let type ← mkForallFVars params type
+          trace[Elab.inductive] "{ctorView.declName} : {type}"
+          return { name := ctorView.declName, type }
+where
+  checkParamOccs (ctorType : Expr) : MetaM Expr :=
+    let visit (e : Expr) : MetaM TransformStep := do
+      let f := e.getAppFn
+      if indFVars.contains f then
+        let mut args := e.getAppArgs
+        unless args.size ≥ params.size do
+          throwError "unexpected inductive type occurrence{indentExpr e}"
+        for i in [:params.size] do
+          let param := params[i]!
+          let arg := args[i]!
+          unless (← isDefEq param arg) do
+            throwError "inductive datatype parameter mismatch{indentExpr arg}\nexpected{indentExpr param}"
+          args := args.set! i param
+        return TransformStep.done (mkAppN f args)
+      else
+        return TransformStep.visit e
+    transform ctorType (pre := visit)
+
+private def getArity (indType : InductiveType) : MetaM Nat :=
+  forallTelescopeReducing indType.type fun xs _ => return xs.size
+private def resetMaskAt (mask : Array Bool) (i : Nat) : Array Bool :=
+  if h : i < mask.size then
+    mask.set ⟨i, h⟩ false
+  else
+    mask
+private def computeFixedIndexBitMask (numParams : Nat) (indType : InductiveType) (indFVars : Array Expr) : MetaM (Array Bool) := do
+  let arity ← getArity indType
+  if arity ≤ numParams then
+    return mkArray arity false
+  else
+    let maskRef ← IO.mkRef (mkArray numParams false ++ mkArray (arity - numParams) true)
+    let rec go (ctors : List Constructor) : MetaM (Array Bool) := do
+      match ctors with
+      | [] => maskRef.get
+      | ctor :: ctors =>
+        forallTelescopeReducing ctor.type fun xs type => do
+          let typeArgs := type.getAppArgs
+          for i in [numParams:arity] do
+            unless i < xs.size && xs[i]! == typeArgs[i]! do -- Remark: if we want to allow arguments to be rearranged, this test should be xs.contains typeArgs[i]
+              maskRef.modify fun mask => mask.set! i false
+          for x in xs[numParams:] do
+            let xType ← inferType x
+            xType.forEach fun e => do
+              if indFVars.any (fun indFVar => e.getAppFn == indFVar) && e.getAppNumArgs > numParams then
+                let eArgs := e.getAppArgs
+                for i in [numParams:eArgs.size] do
+                  if i >= typeArgs.size then
+                    maskRef.modify (resetMaskAt · i)
+                  else
+                    unless eArgs[i]! == typeArgs[i]! do
+                      maskRef.modify (resetMaskAt · i)
+        go ctors
+    go indType.ctors
+
+private def isDomainDefEq (arrowType : Expr) (type : Expr) : MetaM Bool := do
+  if !arrowType.isForall then
+    return false
+  else
+    /-
+      We used to use `withNewMCtxDepth` to make sure we do not assign universe metavariables,
+      but it was not satisfactory. For example, in declarations such as
+      ```
+      inductive Eq : α → α → Prop where
+      | refl (a : α) : Eq a a
+      ```
+      We want the first two indices to be promoted to parameters, and this will only
+      happen if we can assign universe metavariables.
+    -/
+    isDefEq arrowType.bindingDomain! type
+
+private partial def fixedIndicesToParams (numParams : Nat) (indTypes : Array InductiveType) (indFVars : Array Expr) : MetaM Nat := do
+  let masks ← indTypes.mapM (computeFixedIndexBitMask numParams · indFVars)
+  if masks.all fun mask => !mask.contains true then
+    return numParams
+  trace[Elab.inductive] "masks: {masks}"
+  -- We process just a non-fixed prefix of the indices for now. Reason: we don't want to change the order.
+  -- TODO: extend it in the future. For example, it should be reasonable to change
+  -- the order of indices generated by the auto implicit feature.
+  let mask := masks[0]!
+  forallBoundedTelescope indTypes[0]!.type numParams fun params type => do
+    let otherTypes ← indTypes[1:].toArray.mapM fun indType => do whnfD (← instantiateForall indType.type params)
+    let ctorTypes ← indTypes.toList.mapM fun indType => indType.ctors.mapM fun ctor => do whnfD (← instantiateForall ctor.type params)
+    let typesToCheck := otherTypes.toList ++ ctorTypes.join
+    let rec go (i : Nat) (type : Expr) (typesToCheck : List Expr) : MetaM Nat := do
+      if i < mask.size then
+        if !masks.all fun mask => i < mask.size && mask[i]! then
+           return i
+        if !type.isForall then
+          return i
+        let paramType := type.bindingDomain!
+        if !(← typesToCheck.allM fun type => isDomainDefEq type paramType) then
+          trace[Elab.inductive] "domain not def eq: {i}, {type} =?= {paramType}"
+          return i
+        withLocalDeclD `a paramType fun paramNew => do
+          let typesToCheck ← typesToCheck.mapM fun type => whnfD (type.bindingBody!.instantiate1 paramNew)
+          go (i+1) (type.bindingBody!.instantiate1 paramNew) typesToCheck
+      else
+        return i
+    go numParams type typesToCheck
+
+private def getResultingUniverse : List InductiveType → TermElabM Level
+  | []           => throwError "unexpected empty inductive declaration"
+  | indType :: _ => forallTelescopeReducing indType.type fun _ r => do
+    let r ← whnfD r
+    match r with
+    | Expr.sort u => return u
+    | _           => throwError "unexpected inductive type resulting type{indentExpr r}"
+
+private def collectUsed (indTypes : List InductiveType) : StateRefT CollectFVars.State MetaM Unit := do
+  indTypes.forM fun indType => do
+    indType.type.collectFVars
+    indType.ctors.forM fun ctor =>
+      ctor.type.collectFVars
+
+private def removeUnused (vars : Array Expr) (indTypes : List InductiveType) : TermElabM (LocalContext × LocalInstances × Array Expr) := do
+  let (_, used) ← (collectUsed indTypes).run {}
+  Meta.removeUnused vars used
+
+private def withUsed {α} (vars : Array Expr) (indTypes : List InductiveType) (k : Array Expr → TermElabM α) : TermElabM α := do
+  let (lctx, localInsts, vars) ← removeUnused vars indTypes
+  withLCtx lctx localInsts <| k vars
+
+private def updateParams (vars : Array Expr) (indTypes : List InductiveType) : TermElabM (List InductiveType) :=
+  indTypes.mapM fun indType => do
+    let type ← mkForallFVars vars indType.type
+    let ctors ← indType.ctors.mapM fun ctor => do
+      let ctorType ← withExplicitToImplicit vars (mkForallFVars vars ctor.type)
+      return { ctor with type := ctorType }
+    return { indType with type, ctors }
+
+private partial def collectUniverses (views : Array InductiveView) (r : Level) (rOffset : Nat) (numParams : Nat) (indTypes : List InductiveType) : TermElabM (Array Level) := do
+  let (_, us) ← go |>.run #[]
+  return us
+where
+  go : StateRefT (Array Level) TermElabM Unit :=
+    indTypes.forM fun indType => indType.ctors.forM fun ctor =>
+      withCtorRef views ctor.name do
+        forallTelescopeReducing ctor.type fun ctorParams _ =>
+          for ctorParam in ctorParams[numParams:] do
+            accLevelAtCtor ctor ctorParam r rOffset
+
+private def updateResultingUniverse (views : Array InductiveView) (numParams : Nat) (indTypes : List InductiveType) : TermElabM (List InductiveType) := do
+  let r ← getResultingUniverse indTypes
+  let rOffset : Nat   := r.getOffset
+  let r       : Level := r.getLevelOffset
+  unless r.isMVar do
+    throwError "failed to compute resulting universe level of inductive datatype, provide universe explicitly: {r}"
+  let us ← collectUniverses views r rOffset numParams indTypes
+  trace[Elab.inductive] "updateResultingUniverse us: {us}, r: {r}, rOffset: {rOffset}"
+  let rNew := mkResultUniverse us rOffset
+  assignLevelMVar r.mvarId! rNew
+  indTypes.mapM fun indType => do
+    let type ← instantiateMVars indType.type
+    let ctors ← indType.ctors.mapM fun ctor => return { ctor with type := (← instantiateMVars ctor.type) }
+    return { indType with type, ctors }
+
+private def levelMVarToParam (indTypes : List InductiveType) (univToInfer? : Option LMVarId) : TermElabM (List InductiveType) :=
+  go |>.run' 1
+where
+  levelMVarToParam' (type : Expr) : StateRefT Nat TermElabM Expr := do
+    Term.levelMVarToParam' type (except := fun mvarId => univToInfer? == some mvarId)
+
+  go : StateRefT Nat TermElabM (List InductiveType) := do
+    indTypes.mapM fun indType => do
+      let type  ← levelMVarToParam' indType.type
+      let ctors ← indType.ctors.mapM fun ctor => do
+        let ctorType ← levelMVarToParam' ctor.type
+        return { ctor with type := ctorType }
+      return { indType with ctors, type }
+
+private def collectLevelParamsInInductive (indTypes : List InductiveType) : Array Name := Id.run do
+  let mut usedParams : CollectLevelParams.State := {}
+  for indType in indTypes do
+    usedParams := collectLevelParams usedParams indType.type
+    for ctor in indType.ctors do
+      usedParams := collectLevelParams usedParams ctor.type
+  return usedParams.params
+
+private def mkIndFVar2Const (views : Array InductiveView) (indFVars : Array Expr) (levelNames : List Name) : ExprMap Expr := Id.run do
+  let levelParams := levelNames.map mkLevelParam;
+  let mut m : ExprMap Expr := {}
+  for i in [:views.size] do
+    let view    := views[i]!
+    let indFVar := indFVars[i]!
+    m := m.insert indFVar (mkConst view.declName levelParams)
+  return m
+
+private def replaceIndFVarsWithConsts (views : Array InductiveView) (indFVars : Array Expr) (levelNames : List Name)
+    (numVars : Nat) (numParams : Nat) (indTypes : List InductiveType) : TermElabM (List InductiveType) :=
+  let indFVar2Const := mkIndFVar2Const views indFVars levelNames
+  indTypes.mapM fun indType => do
+    let ctors ← indType.ctors.mapM fun ctor => do
+      let type ← forallBoundedTelescope ctor.type numParams fun params type => do
+        let type := type.replace fun e =>
+          if !e.isFVar then
+            none
+          else match indFVar2Const.find? e with
+            | none   => none
+            | some c => mkAppN c (params.extract 0 numVars)
+        instantiateMVars (← mkForallFVars params type)
+      return { ctor with type }
+    return { indType with ctors }
+
+private def mkAuxConstructions (views : Array InductiveView) : TermElabM Unit := do
+  let env ← getEnv
+  let hasEq   := env.contains ``Eq
+  let hasHEq  := env.contains ``HEq
+  let hasUnit := env.contains ``PUnit
+  let hasProd := env.contains ``Prod
+  for view in views do
+    let n := view.declName
+    mkRecOn n
+    if hasUnit then mkCasesOn n
+    if hasUnit && hasEq && hasHEq then mkNoConfusion n
+    if hasUnit && hasProd then mkBelow n
+    if hasUnit && hasProd then mkIBelow n
+  for view in views do
+    let n := view.declName;
+    if hasUnit && hasProd then mkBRecOn n
+    if hasUnit && hasProd then mkBInductionOn n
+
+def addDecl [Monad m] [MonadEnv m] [MonadError m] [MonadOptions m] [MonadLog m] [AddMessageContext m] (decl : Declaration) : m Unit := do
+  if !(← MonadLog.hasErrors) && decl.hasSorry then
+    logWarning "declaration uses 'sorry'"
+  match (← getEnv).addDecl decl with
+  | Except.ok    env => setEnv env
+  | Except.error ex  => throwKernelException ex
+
+private def mkInductiveDecl (vars : Array Expr) (views : Array InductiveView) : TermElabM Unit := Term.withoutSavingRecAppSyntax do
+  let view0 := views[0]!
+  let scopeLevelNames ← Term.getLevelNames
+  -- checkLevelNames views
+  let allUserLevelNames := view0.levelNames
+  let isUnsafe          := view0.modifiers.isUnsafe
+  withRef view0.ref <| Term.withLevelNames allUserLevelNames do
+    let rs ← elabHeader views
+    withInductiveLocalDecls rs fun params indFVars => do
+      trace[Elab.inductive] "indFVars: {indFVars}"
+      let mut indTypesArray : Array InductiveType := #[]
+      for i in [:views.size] do
+        let indFVar := indFVars[i]!
+        Term.addLocalVarInfo views[i]!.declId indFVar
+        let r       := rs[i]!
+        let type  ← mkForallFVars params r.type
+        let ctors ← withExplicitToImplicit params (elabCtors indFVars indFVar params r)
+        indTypesArray := indTypesArray.push { name := r.view.declName, type, ctors }
+      Term.synthesizeSyntheticMVarsNoPostponing
+      let numExplicitParams ← fixedIndicesToParams params.size indTypesArray indFVars
+      trace[Elab.inductive] "numExplicitParams: {numExplicitParams}"
+      let indTypes := indTypesArray.toList
+      let u ← getResultingUniverse indTypes
+      let univToInfer? ← shouldInferResultUniverse u
+      withUsed vars indTypes fun vars => do
+        let numVars   := vars.size
+        let numParams := numVars + numExplicitParams
+        let indTypes ← updateParams vars indTypes
+        let indTypes ← if let some univToInfer := univToInfer? then
+          updateResultingUniverse views numParams (← levelMVarToParam indTypes univToInfer)
+        else
+          -- checkResultingUniverses views numParams indTypes
+          levelMVarToParam indTypes none
+        let usedLevelNames := collectLevelParamsInInductive indTypes
+        match sortDeclLevelParams scopeLevelNames allUserLevelNames usedLevelNames with
+        | .error msg      => throwError msg
+        | .ok levelParams => do
+          let indTypes ← replaceIndFVarsWithConsts views indFVars levelParams numVars numParams indTypes
+          let decl := Declaration.inductDecl levelParams numParams indTypes isUnsafe
+          Term.ensureNoUnassignedMVars decl
+          addDecl decl
+          mkAuxConstructions views
+    withSaveInfoContext do  -- save new env
+      for view in views do
+        Term.addTermInfo' view.ref[1] (← mkConstWithLevelParams view.declName) (isBinder := true)
+        for ctor in view.ctors do
+          Term.addTermInfo' ctor.ref[2] (← mkConstWithLevelParams ctor.declName) (isBinder := true)
+        -- We need to invoke `applyAttributes` because `class` is implemented as an attribute.
+        Term.applyAttributesAt view.declName view.modifiers.attrs .afterTypeChecking
+
+/-
+Paper that describes writing custom parser:
+https://eprints.illc.uva.nl/id/eprint/2239/1/MoL-2023-03.text.pdf
+GitHub: https://github.com/alexkeizer/qpf4
+-/
+def Lean.Parser.Command.«bad_inductive» := leading_parser "bad_inductive " >> Lean.Parser.Command.declId >> Lean.Parser.Command.optDeclSig >> Lean.Parser.many Lean.Parser.Command.ctor
+@[commandParser] def declaration := leading_parser
+Lean.Parser.Command.declModifiers false >> Lean.Parser.Command.«bad_inductive»
+
+-- @[builtinCommandElab declaration]
+def elabDeclaration' : CommandElab := fun stx => do
+  let decl     := stx[1]
+  let declKind := decl.getKind
+  if declKind == ``Lean.Parser.Command.«bad_inductive» then
+    let modifiers ← elabModifiers stx[0]
+    elabInductive modifiers decl
+  else
+    throwError "unexpected declaration"
+
+private def applyComputedFields (indViews : Array InductiveView) : CommandElabM Unit := do
+  if indViews.all (·.computedFields.isEmpty) then return
+
+  let mut computedFields := #[]
+  let mut computedFieldDefs := #[]
+  for indView@{declName, ..} in indViews do
+    for {ref, fieldId, type, matchAlts, modifiers, ..} in indView.computedFields do
+      computedFieldDefs := computedFieldDefs.push <| ← do
+        let modifiers ← match modifiers with
+          | `(Lean.Parser.Command.declModifiersT| $[$doc:docComment]? $[$attrs:attributes]? $[$vis]? $[noncomputable]?) =>
+            `(Lean.Parser.Command.declModifiersT| $[$doc]? $[$attrs]? $[$vis]? noncomputable)
+          | _ => do
+            withRef modifiers do logError "unsupported modifiers for computed field"
+            `(Parser.Command.declModifiersT| noncomputable)
+        `($(⟨modifiers⟩):declModifiers
+          def%$ref $(mkIdent <| `_root_ ++ declName ++ fieldId):ident : $type $matchAlts:matchAlts)
+    let computedFieldNames := indView.computedFields.map fun {fieldId, ..} => declName ++ fieldId
+    computedFields := computedFields.push (declName, computedFieldNames)
+  withScope (fun scope => { scope with
+      opts := scope.opts
+        |>.setBool `bootstrap.genMatcherCode false
+        |>.setBool `elaboratingComputedFields true}) <|
+    elabCommand <| ← `(mutual $computedFieldDefs* end)
+
+  liftTermElabM do Term.withDeclName indViews[0]!.declName do
+    ComputedFields.setComputedFields computedFields
+
+private def applyDerivingHandlers (views : Array InductiveView) : CommandElabM Unit := do
+  let mut processed : NameSet := {}
+  for view in views do
+    for classView in view.derivingClasses do
+      let className := classView.className
+      unless processed.contains className do
+        processed := processed.insert className
+        let mut declNames := #[]
+        for view in views do
+          if view.derivingClasses.any fun classView => classView.className == className then
+            declNames := declNames.push view.declName
+        classView.applyHandlers declNames
+
+def elabInductiveViewsUnsafe (views : Array InductiveView) : CommandElabM Unit := do
+  let view0 := views[0]!
+  let ref := view0.ref
+  runTermElabM fun vars => Term.withDeclName view0.declName do withRef ref do
+    mkInductiveDecl vars views
+    mkSizeOfInstances view0.declName
+    Lean.Meta.IndPredBelow.mkBelow view0.declName
+    for view in views do
+      mkInjectiveTheorems view.declName
+  applyComputedFields views -- NOTE: any generated code before this line is invalid
+  applyDerivingHandlers views
+  runTermElabM fun _ => Term.withDeclName view0.declName do withRef ref do
+    for view in views do
+      Term.applyAttributesAt view.declName view.modifiers.attrs .afterCompilation
+
+@[commandElab declaration]
+def elabData : CommandElab := fun stx => do
+  let modifiers ← elabModifiers stx[0]
+  let decl := stx[1]
+  -- dbg_trace decl
+  let view ← badInductiveSyntaxToView modifiers decl
+  -- elabInductiveViews #[view]
+  elabInductiveViewsUnsafe #[view]
+
+#check InductiveView
+bad_inductive test : Type
+| a: test
+| b : test
+| c : test → test
+
+bad_inductive Bad : Type
+| a : Type → Bad
+
+#check @test.rec
+
+#check test.a
+
+def x : test → Nat
+| .a => 0
+| .b => 1
+| .c q => x q + 1
+
+-- #eval test `(inductive thing : Type | x : thing)
+
+------------------------------------------------------------------------
+#check Lean.Elab.Term.elabMatch
+
+@[builtinTermParser] def «match_with_axioms» := leading_parser:Lean.Parser.leadPrec "«match_with_axioms» " >> Lean.Parser.optional Lean.Parser.Term.generalizingParam >> Lean.Parser.optional Lean.Parser.Term.motive >> Lean.Parser.sepBy1 Lean.Parser.Term.matchDiscr ", " >> " with " >> Lean.Parser.ppDedent Lean.Parser.Term.matchAlts
+@[commandParser] def match_decl := leading_parser
+Lean.Parser.Command.declModifiers false >> «match_with_axioms»
+
+@[commandElab match_decl]
+def elabMatch : TermElab := fun stx expectedType? => do
+  sorry
